---
title: "Variance of a Binomial"
author: "Joshua Wiseman"
date: "`r Sys.Date()`"
output: 
  html_document: 
    toc: yes
    toc_float: yes
---

```{r setup, include=FALSE}
knitr::opts_chunk$set(echo = TRUE, message = FALSE)
```

# Introduction

We have learnt that the MGF for a binomial random variable is:

$$M_X(t) = (q+pe^t)^n $$

Where $X\sim Bin(n,p)$

# Tasks

Using the moment generating function above prove that 

$$\sigma^2 = npq$$

by answering the tasks below. 
Use $\LaTeX$ to construct the proof for Task 1.

## Task 1

Start with 

$$
\begin{eqnarray}
E(X) &=& \left . \frac{d M_X(t)}{dt}\right |_{t=0}\\
E(X) &=& \frac{d}{dt} (q+pe^t)^n |_{t=0}\\
E(X) &=& npe^t(q+pe^t)^{n-1} |_{t=0}\\
E(X) &=& npe^0(q+pe^0)^{n-1}\\
E(X) &=& np(q+p)^{n-1}\\
E(X) &=& np(1)^{n-1}\\
E(X) &=& np\\
\mu &=& np
\end{eqnarray}
$$

## Task 2

You may use paper and write neatly the proof - take a picture and place in the document using 

`![](){}`

Now find $E(X^2)$

$$
\begin{eqnarray}
E(X^2) &=& \left . \frac{d^2 M_X(t)}{dt^2}\right |_{t=0}\\
&=& \frac{d^2}{dt^2} (q+pe^t)^n |_{t=0}\\
&=& \frac{d}{dt} npe^t(q+pe^t)^{n-1}|_{t=0}\\
&=& npe^t(q+pe^t)^{n-1} + (n-1)np^2e^{2t}(q+pe^t)^{n-2} |_{t=0}\\
&=& npe^0(q+pe^0)^{n-1} + (n-1)np^2e^{2*0}(q+pe^0)^{n-2}\\
&=& np(q+p)^{n-1} + (n-1)np^2(q+p)^{n-2}\\
&=& np(1)^{n-1} + (n-1)np^2(1)^{n-2}\\
&=& np + (n-1)np^2\\
&=& np + n^2p^2 - np^2\\
&=& np(1 + np - p)\\
&=& np(q + np)\\
\end{eqnarray}
$$

## Task 3

Find $\sigma^2$ Using the formula $\sigma^2 =E(X^2)-\mu^2$

$$
\begin{eqnarray}
\sigma^2 &=& E(X^2)-\mu^2\\
E(X^2) &=& np(q + np)\\
\mu &=& np\\
\sigma^2 &=& np(q + np) - (np)^2\\
&=& npq + (np)^2 - (np)^2\\
&=& npq
\end{eqnarray}
$$
